Through up to half of Lambda

theories/Substitution/Introductions/Pi.v
@@ -1,8 +1,8 @@
 From Coq Require Import ssrbool.
 From LogRel.AutoSubst Require Import core unscoped Ast Extra.
-From LogRel Require Import Utils BasicAst Notations Context NormalForms Weakening
-  GenericTyping LogicalRelation Validity.
-From LogRel.LogicalRelation Require Import Escape Reflexivity Neutral Weakening Irrelevance.
+From LogRel Require Import Utils BasicAst Notations LContexts Context NormalForms Weakening
+  GenericTyping Monad LogicalRelation Validity.
+From LogRel.LogicalRelation Require Import Escape Reflexivity Neutral Weakening Split Irrelevance.
 From LogRel.Substitution Require Import Irrelevance Properties.
 From LogRel.Substitution.Introductions Require Import Universe Poly.
 
@@ -21,38 +21,40 @@ Qed. *)
 Section PolyRedPi.
   Context `{GenericTypingProperties}.
 
-  Lemma LRPiPoly0 {Γ l A B} (PAB : PolyRed Γ l A B) : [Γ ||-Π<l> tProd A B].
+  Lemma LRPiPoly0 {wl Γ l A B} (PAB : PolyRed wl Γ l A B) : [Γ ||-Π<l> tProd A B]< wl >.
   Proof.
     econstructor; tea; pose proof (polyRedId PAB) as []; escape.
-    + eapply redtywf_refl; gen_typing.
+    + eapply redtywf_refl ; Wescape ; gen_typing.
     + unshelve eapply escapeEq; tea; eapply reflLRTyEq.
-    + eapply convty_prod; tea; unshelve eapply escapeEq; tea; eapply reflLRTyEq.
+    + cbn ; Wescape ; eapply convty_prod; tea.
+      * unshelve eapply escapeEq ; tea ; now eapply reflLRTyEq.
+      * unshelve eapply WescapeEq ; tea ; now eapply WreflLRTyEq.
   Defined.
 
-  Definition LRPiPoly {Γ l A B} (PAB : PolyRed Γ l A B) : [Γ ||-<l> tProd A B] := LRPi' (LRPiPoly0 PAB).
+  Definition LRPiPoly {wl Γ l A B} (PAB : PolyRed wl Γ l A B) : [Γ ||-<l> tProd A B]< wl > := LRPi' (LRPiPoly0 PAB).
 
-  Lemma LRPiPolyEq0 {Γ l A A' B B'} (PAB : PolyRed Γ l A B) (Peq : PolyRedEq PAB A' B') :
-    [Γ |- A'] -> [Γ ,, A' |- B'] ->
-    [Γ ||-Π tProd A B ≅ tProd A' B' | LRPiPoly0 PAB].
+  Lemma LRPiPolyEq0 {wl Γ l A A' B B'} (PAB : PolyRed wl Γ l A B) (Peq : PolyRedEq PAB A' B') :
+    [Γ |- A']< wl > -> [Γ ,, A' |- B']< wl > ->
+    [Γ ||-Π tProd A B ≅ tProd A' B' | LRPiPoly0 PAB]< wl >.
   Proof.
     econstructor; cbn; tea.
     + eapply redtywf_refl; gen_typing.
     + pose proof (polyRedEqId PAB Peq) as []; now escape.
-    + pose proof (polyRedEqId PAB Peq) as []; escape.
+    + pose proof (polyRedEqId PAB Peq) as []; escape ; Wescape.
       eapply convty_prod; tea.
       eapply escape; now apply (polyRedId PAB).
   Qed.
 
-  Lemma LRPiPolyEq {Γ l A A' B B'} (PAB : PolyRed Γ l A B) (Peq : PolyRedEq PAB A' B') :
-    [Γ |- A'] -> [Γ ,, A' |- B'] ->
-    [Γ ||-<l> tProd A B ≅ tProd A' B' | LRPiPoly PAB].
+  Lemma LRPiPolyEq {wl Γ l A A' B B'} (PAB : PolyRed wl Γ l A B) (Peq : PolyRedEq PAB A' B') :
+    [Γ |- A']< wl > -> [Γ ,, A' |- B']< wl > ->
+    [Γ ||-<l> tProd A B ≅ tProd A' B' | LRPiPoly PAB]< wl >.
   Proof.
     now eapply LRPiPolyEq0.
   Qed.
 
-  Lemma LRPiPolyEq' {Γ l A A' B B'} (PAB : PolyRed Γ l A B) (Peq : PolyRedEq PAB A' B') (RAB : [Γ ||-<l> tProd A B]):
-    [Γ |- A'] -> [Γ ,, A' |- B'] ->
-    [Γ ||-<l> tProd A B ≅ tProd A' B' | RAB].
+  Lemma LRPiPolyEq' {wl Γ l A A' B B'} (PAB : PolyRed wl Γ l A B) (Peq : PolyRedEq PAB A' B') (RAB : [Γ ||-<l> tProd A B]< wl >):
+    [Γ |- A']< wl > -> [Γ ,, A' |- B']< wl > ->
+    [Γ ||-<l> tProd A B ≅ tProd A' B' | RAB]< wl >.
   Proof.
     intros; irrelevanceRefl; now eapply LRPiPolyEq.
   Qed.
@@ -63,44 +65,58 @@ End PolyRedPi.
 Section PiTyValidity.
 
   Context `{GenericTypingProperties}.
-  Context {l Γ F G} (vΓ : [||-v Γ])
-    (vF : [Γ ||-v< l > F | vΓ ])
-    (vG : [Γ ,, F ||-v< l > G | validSnoc vΓ vF]).
+  Context {l wl Γ F G} (vΓ : [||-v Γ]< wl >)
+    (vF : [Γ ||-v< l > F | vΓ ]< wl >)
+    (vG : [Γ ,, F ||-v< l > G | validSnoc' vΓ vF]< wl >).
 
-  Lemma PiRed {Δ σ} (tΔ : [ |-[ ta ] Δ])
-    (vσ : [vΓ | Δ ||-v σ : _ | tΔ])
-    : [ Δ ||-< l > (tProd F G)[σ] ].
+  Lemma PiRed {Δ σ wl'} f (tΔ : [ |-[ ta ] Δ]< wl' >)
+    (vσ : [vΓ | Δ ||-v σ : _ | tΔ | f]< wl >)
+    : W[ Δ ||-< l > (tProd F G)[σ] ]< wl' >.
   Proof.
+    pose (p := substPolyRed vΓ vF vG _ vσ).
+    exists (WPol _ _ _ _ _ p) ; intros wl'' Hover.
+    pose proof (over_tree_le Hover).
     eapply LRPi'.
-    pose (p := substPolyRed vΓ vF vG _ vσ).
-    escape; cbn; econstructor; tea;
-    destruct (polyRedId p);
-    destruct (polyRedEqId p (substPolyRedEq vΓ vF vG _ vσ vσ (reflSubst _ _ vσ))); escape.
-    - apply redtywf_refl; gen_typing.
-    - gen_typing.
-    - gen_typing.
+
+    destruct (WpolyRedId p);
+      destruct (WpolyRedEqId p (substPolyRedEq vΓ vF vG _ vσ vσ (reflSubst _ _ _ vσ))); Wescape.
+    cbn ; econstructor; tea.
+    - eapply redtywf_refl, wft_Ltrans ; [eassumption | gen_typing].
+    - eapply convty_Ltrans ; [eassumption | gen_typing].
+    - eapply convty_Ltrans ; [eassumption | gen_typing].
+    - now eapply p.
   Defined.
 
-  Lemma PiEqRed1 {Δ σ σ'} (tΔ : [ |-[ ta ] Δ])
-    (vσ : [vΓ | Δ ||-v σ : _ | tΔ])
-    (vσ' : [vΓ | Δ ||-v σ' : _ | tΔ])
-    (vσσ' : [vΓ | Δ ||-v σ ≅ σ' : _ | tΔ | vσ])
-    : [ Δ ||-< l > (tProd F G)[σ] ≅ (tProd F G)[σ'] | PiRed tΔ vσ ].
+  Lemma PiEqRed1 {Δ σ σ' wl' f} (tΔ : [ |-[ ta ] Δ]< wl' >)
+    (vσ : [vΓ | Δ ||-v σ : _ | tΔ | f]< wl >)
+    (vσ' : [vΓ | Δ ||-v σ' : _ | tΔ | f]< wl >)
+    (vσσ' : [vΓ | Δ ||-v σ ≅ σ' : _ | tΔ | vσ | f]< wl >)
+    : W[ Δ ||-< l > (tProd F G)[σ] ≅ (tProd F G)[σ'] | PiRed f tΔ vσ ]< wl' >.
   Proof.
-    pose (p := substPolyRed vΓ vF vG _ vσ).
-    pose (p' := substPolyRed vΓ vF vG _ vσ').
-    pose (peq := substPolyRedEq vΓ vF vG _ vσ vσ' vσσ').
-    destruct (polyRedId p); destruct (polyRedId p'); destruct (polyRedEqId p peq).
-    escape; econstructor; cbn; tea.
-    - apply redtywf_refl; gen_typing.
-    - gen_typing.
+    unfold PiRed ; cbn.
+    set (p := substPolyRed vΓ vF vG _ vσ).
+    set (p' := substPolyRed vΓ vF vG _ vσ').
+    destruct (WpolyRedEqId p (substPolyRedEq vΓ vF vG tΔ vσ vσ (reflSubst vΓ f tΔ vσ))) as [Q1 Q2] ; cbn.
+    set (peq := substPolyRedEq vΓ vF vG _ vσ vσ' vσσ').
+    destruct (WpolyRedId p); destruct (WpolyRedId p'); destruct (WpolyRedEqId p peq).
+    cbn.
+    unfold PiRed.
+    exists (WPolEq _ _ _ peq).
+    cbn.
+    intros wl'' Hover Hover'.
+    Wescape; econstructor ; cbn ; tea.
+    - eapply redtywf_refl, wft_Ltrans ; [ now eapply over_tree_le | gen_typing].
+    - eapply convty_Ltrans ; [ now eapply over_tree_le | gen_typing].
+    - eapply convty_Ltrans ; [ now eapply over_tree_le | gen_typing].
+    - eapply peq.
+      assumption.
   Defined.
 
-  Lemma PiValid : [Γ ||-v< l > tProd F G | vΓ].
+  Lemma PiValid : [Γ ||-v< l > tProd F G | vΓ]< wl >.
   Proof.
     unshelve econstructor.
-    - intros Δ σ. eapply PiRed.
-    - intros Δ σ σ'. eapply PiEqRed1.
+    - intros Δ wl' σ. eapply PiRed.
+    - intros Δ wl' σ σ' f. eapply PiEqRed1.
   Defined.
 
 End PiTyValidity.
@@ -108,29 +124,35 @@ End PiTyValidity.
 Section PiTyDomValidity.
 
   Context `{GenericTypingProperties}.
-  Context {l Γ F G} (vΓ : [||-v Γ])
-    (vΠFG : [Γ ||-v< l > tProd F G | vΓ ]).
+  Context {l wl Γ F G} (vΓ : [||-v Γ]< wl >)
+    (vΠFG : [Γ ||-v< l > tProd F G | vΓ ]< wl >).
 
-  Lemma PiValidDom : [Γ ||-v< l > F | vΓ].
+  Lemma PiValidDom : [Γ ||-v< l > F | vΓ]< wl >.
   Proof.
   unshelve econstructor.
-  - intros Δ σ vΔ vσ; instValid vσ.
-    cbn in RvΠFG; apply Induction.invLRΠ in RvΠFG.
-    destruct RvΠFG as [dom ? red ? ? ? [? ? Hdom]].
+  - intros Δ wl' σ f vΔ vσ ; instValid vσ.
+    exists (WT _ (validTy vΠFG f vΔ vσ)).
+    intros wl'' Hover.
+    pose (Help := WRed _ (validTy vΠFG f vΔ vσ) wl'' Hover).
+    cbn in RvΠFG; apply Induction.invLRΠ in Help ; fold subst_term in Help.
+    destruct Help as [dom ? red ? ? ? [? ? Hdom]].
     assert (Hrw : F[σ] = dom); [|subst dom].
     { eapply redtywf_whnf in red as [=]; [tea|constructor]. }
     rewrite <- (wk_id_ren_on Δ F[σ]).
-    now eapply Hdom.
-  - cbn; refold.
-    intros Δ σ σ' vΔ vσ vσ' vσσ'.
-    match goal with |- [ LRAd.pack ?P | _ ||- _ ≅ _] => set (vF := P); clearbody vF end.
-    instValid vσ.
-    cbn in RvΠFG; apply Induction.invLRΠ in RvΠFG.
-    assert (vΠ := validTyExt vΠFG _ vσ vσ' vσσ').
-    eapply LRTyEqIrrelevant' with (lrA' := LRPi' RvΠFG) in vΠ; [|reflexivity].
-    destruct RvΠFG as [dom ? red ? ? ? []].
-    destruct vΠ as [dom' ? red' ? ? [Heq _]]; simpl in *.
-    specialize (Heq Δ wk_id vΔ).
+    eapply Hdom ; [ now eapply wfLCon_le_id | eapply wfc_Ltrans ; eauto].
+    now eapply over_tree_le.
+  - intros Δ wl' σ σ' f vΔ vσ vσ' vσσ'.
+    cbn; refold.
+    assert (vΠ := validTyExt vΠFG _ _ vσ vσ' vσσ').
+    exists (WTEq _ vΠ).
+    cbn ; refold ; intros wl'' Hover Hover'.
+    pose (Help := WRed _ (validTy vΠFG f vΔ vσ) wl'' Hover).
+    apply Induction.invLRΠ in Help ; fold subst_term in Help.
+    pose (Help2 := WRedEq _ vΠ wl'' Hover Hover').
+    eapply LRTyEqIrrelevant' with (lrA' := LRPi' Help) in Help2 ; [|reflexivity].
+    destruct Help as [dom ? red ? ? ? []].
+    destruct Help2 as [dom' ? red' ? ? [Heq]]; simpl in *.
+    specialize (Heq Δ wk_id _ (idε _) (wfc_Ltrans (over_tree_le Hover) vΔ)).
     assert (Hrw : F[σ] = dom).
     { eapply redtywf_whnf in red as [=]; [tea|constructor]. }
     assert (Hrw' : F[σ'] = dom').
@@ -138,37 +160,59 @@ Section PiTyDomValidity.
     rewrite wk_id_ren_on, <- Hrw' in Heq.
     eapply Transitivity.transEq; [|eapply Heq].
     rewrite <- (wk_id_ren_on Δ dom) in Hrw; rewrite <- Hrw.
-    eapply LRTyEqIrrelevant' with (lrA := vF); [reflexivity|].
-    eapply reflLRTyEq.
+    now eapply reflLRTyEq.
   Qed.
 
-  Lemma PiValidCod : [Γ,, F ||-v< l > G | validSnoc vΓ PiValidDom].
+  Lemma PiValidCod : [Γ,, F ||-v< l > G | validSnoc' vΓ PiValidDom]< wl >.
   Proof.
   unshelve econstructor.
-  - intros Δ σ vΔ [vσ v0].
+  - intros Δ wl' σ f vΔ [vσ v0].
     instValid vσ; cbn in *.
-    apply Induction.invLRΠ in RvΠFG.
-    destruct RvΠFG as [dom cod red ? ? ? [? ? Hdom Hcod _]].
-    specialize (Hcod Δ (σ 0) wk_id vΔ).
-    assert (HF : F[↑ >> σ] = dom).
-    { eapply redtywf_whnf in red as [=]; [tea|constructor]. }
-    assert (HG0 : G[up_term_term (↑ >> σ)] = cod).
-    { eapply redtywf_whnf in red as [=]; [tea|constructor]. }
-    assert (HG : G[σ] = cod[σ 0 .: @wk_id Δ >> tRel]).
-    { rewrite <- HG0; bsimpl; apply ext_term; intros []; reflexivity. }
-    rewrite HG; apply Hcod.
-    irrelevance0; [|eapply v0].
-    now rewrite wk_id_ren_on.
-  - cbn; refold.
-    intros Δ σ σ' vΔ [vσ v0] [vσ' v0'] [vσσ' v00'].
-    match goal with |- [ LRAd.pack ?P | _ ||- _ ≅ _] => set (vG := P); clearbody vG end.
+    unshelve eapply TreeSplit.
+    + eapply DTree_fusion ; [eapply DTree_fusion | exact (WTTm _ v0)].
+      * exact (WT _ (validTy PiValidDom f vΔ vσ)).
+      * exact (WT _ RvΠFG).
+    + intros wl'' Hover.
+      pose (Ho := over_tree_fusion_l (over_tree_fusion_l Hover)).
+      pose (Ho' := over_tree_fusion_r (over_tree_fusion_l Hover)).
+      pose (Ho'' := over_tree_fusion_r Hover).
+      pose (Help:= WRed _ RvΠFG _ Ho').
+      apply Induction.invLRΠ in Help.
+      destruct Help as [dom cod red ? ? ? [? ? Hdom ? Hcod _ _]].
+      specialize (Hcod Δ (σ 0) wl'' wk_id (idε _) (wfc_Ltrans (over_tree_le Hover) vΔ)).
+      assert (HF : F[↑ >> σ] = dom).
+      { eapply redtywf_whnf in red as [=]; [tea|constructor]. }
+      assert (HG0 : G[up_term_term (↑ >> σ)] = cod).
+      { eapply redtywf_whnf in red as [=]; [tea|constructor]. }
+      assert (HG : G[σ] = cod[σ 0 .: @wk_id Δ >> tRel]).
+      { rewrite <- HG0; bsimpl; apply ext_term; intros []; reflexivity. }
+      rewrite HG.
+      econstructor.
+      intros wl''' Hover' ; eapply Hcod.
+      exact Hover'.
+      Unshelve. irrelevance0; [|unshelve eapply v0 ; eauto].
+      now rewrite wk_id_ren_on.
+  - intros Δ wl' σ σ' f vΔ [vσ v0] [vσ' v0'] [vσσ' v00'].
+    cbn; refold.
+    assert (vΠ := validTyExt vΠFG _ _ vσ vσ' vσσ').
     instValid vσ.
-    cbn in RvΠFG; apply Induction.invLRΠ in RvΠFG.
-    assert (vΠ := validTyExt vΠFG _ vσ vσ' vσσ').
-    eapply LRTyEqIrrelevant' with (lrA' := LRPi' RvΠFG) in vΠ; [|reflexivity].
-    destruct RvΠFG as [dom cod red ? ? ? [? ? ? ? Hcod]].
-    destruct vΠ as [dom' cod' red' ? ? [Hdom' Hcod']]; simpl in *.
-    specialize (Hcod' Δ (σ' 0) wk_id vΔ).
+    eapply TreeEqSplit.
+    intros wl'' Hover HGRed.
+    epose (Ho := over_tree_fusion_l (over_tree_fusion_l (over_tree_fusion_l Hover))).
+    epose (Ho' := over_tree_fusion_r (over_tree_fusion_l (over_tree_fusion_l Hover))).
+    epose (Ho2 := over_tree_fusion_l (over_tree_fusion_r (over_tree_fusion_l Hover))).
+    epose (Ho3 := over_tree_fusion_r (over_tree_fusion_r (over_tree_fusion_l Hover))).
+    epose (Ho4 := over_tree_fusion_l (over_tree_fusion_l (over_tree_fusion_r Hover))).
+    epose (Ho5 := over_tree_fusion_r (over_tree_fusion_l (over_tree_fusion_r Hover))).
+    epose (Ho6 := over_tree_fusion_l (over_tree_fusion_r (over_tree_fusion_r Hover))).
+    epose (Ho7 := over_tree_fusion_r (over_tree_fusion_r (over_tree_fusion_r Hover))).
+    pose (Help := WRed _ RvΠFG _ Ho).
+    pose (Help2 := WRedEq _ vΠ _ Ho' Ho2).
+    cbn in Help; apply Induction.invLRΠ in Help.
+    eapply LRTyEqIrrelevant' with (lrA' := LRPi' Help) in Help2; [|reflexivity].
+    destruct Help as [dom cod red ? ? ? [? ? ? ? ? ? Hcod]].
+    destruct Help2 as [dom' cod' red' ? ? [Hdom' ? Hcod']]; simpl in *.
+    specialize (Hcod' Δ (σ' 0) _ wk_id (idε _) (wfc_Ltrans (over_tree_le Ho) vΔ)).
     assert (HF : F[↑ >> σ] = dom).
     { eapply redtywf_whnf in red as [=]; [tea|constructor]. }
     assert (HF' : F[↑ >> σ'] = dom').
@@ -182,22 +226,35 @@ Section PiTyDomValidity.
     assert (HG' : G[σ'] = cod'[σ' 0 .: @wk_id Δ >> tRel]).
     { rewrite <- HG0'; bsimpl; apply ext_term; intros []; reflexivity. }
     rewrite HG'.
-    assert (Hσ0 : [shpRed Δ wk_id vΔ | _ ||- σ 0 : _]).
-    { irrelevance0; [|eapply v0].
+    assert (Hσ0 : [shpRed Δ wl'' wk_id ((idε) wl'') (wfc_Ltrans (over_tree_le Ho) vΔ) | _ ||- σ 0 : _]< wl'' >).
+    { irrelevance0; [| unshelve eapply v0 ; [exact Ho3 | exact Ho4 ]].
       now rewrite wk_id_ren_on. }
-    assert (Hσ0' : [shpRed Δ wk_id vΔ | _ ||- σ' 0 : _]).
-    { eapply LRTmRedConv; [|eapply v0'].
+    assert (Hσ0' : [shpRed Δ wl'' wk_id ((idε) wl'') (wfc_Ltrans (over_tree_le Ho) vΔ) | _ ||- σ' 0 : _]< wl'' >).
+    { eapply LRTmRedConv; [|unshelve eapply v0' ; [exact Ho5 | exact Ho6] ].
       eapply LRTyEqSym; rewrite HF'.
       rewrite <- (wk_id_ren_on Δ dom').
-      apply (Hdom' _ _ vΔ). }
-    eassert (Hcod0 := Hcod Δ (σ 0) (σ' 0) wk_id vΔ Hσ0 Hσ0').
-    eapply Transitivity.transEq; [|now unshelve eapply Hcod'].
+      unshelve eapply Hdom' ; [exact ((idε) wl'') | ].
+      exact (wfc_Ltrans (over_tree_le Ho) vΔ).
+    }
+    eassert (Hcod0 := Hcod Δ _ (σ 0) (σ' 0) wk_id ((idε) wl'') (wfc_Ltrans (over_tree_le Ho) vΔ) Hσ0 Hσ0').
+    econstructor.
+    intros wl''' Hover' Hover''.
+    eapply Transitivity.transEq; [| unshelve eapply Hcod'].
     eapply Transitivity.transEq; [|unshelve eapply Hcod0].
-    + unshelve (irrelevance0; [|eapply reflLRTyEq]); try now symmetry.
-      shelve.
-      now eauto.
-    + irrelevance0; [|eapply v00'].
-      now rewrite wk_id_ren_on.
+    1:{ unshelve (irrelevance0; [|eapply reflLRTyEq]); try now symmetry.
+        shelve.
+        unshelve eapply posRed.
+        4: eauto.
+        eapply over_tree_fusion_l ; exact Hover''.
+    }
+    2:{ irrelevance0; [| unshelve eapply v00' ; auto ; exact Ho7].
+        now rewrite wk_id_ren_on.
+    }
+    1: now eapply over_tree_fusion_l.
+    3: eauto.
+    1,3: eapply over_tree_fusion_l, over_tree_fusion_r ; exact Hover''.
+    1: do 3 (eapply over_tree_fusion_r) ; exact Hover''.
+    eapply over_tree_fusion_l, over_tree_fusion_r, over_tree_fusion_r ; exact Hover''.
   Qed.
 
 End PiTyDomValidity.
@@ -205,30 +262,41 @@ End PiTyDomValidity.
 Section PiTyCongruence.
 
   Context `{GenericTypingProperties}.
-  Context {Γ F G F' G' l}
-    (vΓ : [||-v Γ])
-    (vF : [ Γ ||-v< l > F | vΓ ])
-    (vG : [ Γ ,, F ||-v< l > G | validSnoc vΓ vF ])
-    (vF' : [ Γ ||-v< l > F' | vΓ ])
-    (vG' : [ Γ ,, F' ||-v< l > G' | validSnoc vΓ vF' ])
-    (vFF' : [ Γ ||-v< l > F ≅ F' | vΓ | vF ])
-    (vGG' : [ Γ ,, F ||-v< l > G ≅ G' | validSnoc vΓ vF | vG ]).
+  Context {wl Γ F G F' G' l}
+    (vΓ : [||-v Γ]< wl >)
+    (vF : [ Γ ||-v< l > F | vΓ ]< wl >)
+    (vG : [ Γ ,, F ||-v< l > G | validSnoc' vΓ vF ]< wl >)
+    (vF' : [ Γ ||-v< l > F' | vΓ ]< wl >)
+    (vG' : [ Γ ,, F' ||-v< l > G' | validSnoc' vΓ vF' ]< wl >)
+    (vFF' : [ Γ ||-v< l > F ≅ F' | vΓ | vF ]< wl >)
+    (vGG' : [ Γ ,, F ||-v< l > G ≅ G' | validSnoc' vΓ vF | vG ]< wl >).
 
-  Lemma PiEqRed2 {Δ σ} (tΔ : [ |-[ ta ] Δ]) (vσ : [vΓ | Δ ||-v σ : _ | tΔ])
-    : [ Δ ||-< l > (tProd F G)[σ] ≅ (tProd F' G')[σ] | validTy (PiValid vΓ vF vG) tΔ vσ ].
+  Lemma PiEqRed2 {Δ σ wl' f} (tΔ : [ |-[ ta ] Δ]< wl' >) (vσ : [vΓ | Δ ||-v σ : _ | tΔ | f]< wl >)
+    : W[ Δ ||-< l > (tProd F G)[σ] ≅ (tProd F' G')[σ] | validTy (PiValid vΓ vF vG) f tΔ vσ ]< wl' >.
   Proof.
-    pose (p := substPolyRed vΓ vF vG _ vσ).
-    pose (p' := substPolyRed vΓ vF' vG' _ vσ).
-    pose (peq := substEqPolyRedEq vΓ vF vG _ vσ vF' vG' vFF' vGG').
-    destruct (polyRedId p); destruct (polyRedId p'); destruct (polyRedEqId p peq).
-    escape; econstructor; cbn; tea.
-    - apply redtywf_refl; gen_typing.
-    - gen_typing.
+    unfold PiValid, PiRed ; cbn.
+    set (p := substPolyRed vΓ vF vG _ vσ).
+    set (p' := substPolyRed vΓ vF' vG' _ vσ).
+    set (peq := substEqPolyRedEq vΓ vF vG _ vσ vF' vG' vFF' vGG').
+    set (peq' := (substPolyRedEq vΓ vF vG tΔ vσ vσ (reflSubst vΓ f tΔ vσ))).
+    destruct (WpolyRedEqId p peq') ; cbn.
+    destruct (WpolyRedId p); destruct (WpolyRedId p') ; destruct (WpolyRedEqId p peq) ; cbn.
+    Wescape; cbn; tea.
+    econstructor ; intros wl'' Hover Hover'; cbn.
+    econstructor ; cbn in *.
+    - eapply redtywf_refl, wft_Ltrans ; [now eapply (over_tree_le Hover) | ].
+      gen_typing.
+    - eapply convty_Ltrans ; [ now eapply over_tree_le | ] ; cbn.
+      now gen_typing.
+    - eapply convty_Ltrans ; [ now eapply over_tree_le | ] ; cbn.
+      now gen_typing.
+    - eapply peq.
+      exact Hover'.
   Qed.
 
-  Lemma PiCong : [ Γ ||-v< l > tProd F G ≅ tProd F' G' | vΓ | PiValid vΓ vF vG ].
+  Lemma PiCong : [ Γ ||-v< l > tProd F G ≅ tProd F' G' | vΓ | PiValid vΓ vF vG ]< wl >.
   Proof.
-    econstructor. intros Δ σ. eapply PiEqRed2.
+    econstructor. intros Δ wl' σ f. eapply PiEqRed2.
   Qed.
 
 End PiTyCongruence.
@@ -237,60 +305,74 @@ End PiTyCongruence.
 Section PiTmValidity.
 
   Context `{GenericTypingProperties}.
-  Context {Γ F G} (VΓ : [||-v Γ])
-    (VF : [ Γ ||-v< one > F | VΓ ])
-    (VU : [ Γ ,, F ||-v< one > U | validSnoc VΓ VF ])
-    (VFU : [ Γ ||-v< one > F : U | VΓ | UValid VΓ ])
-    (VGU : [ Γ ,, F ||-v< one > G : U | validSnoc VΓ VF | VU ]) .
+  Context {wl Γ F G} (VΓ : [||-v Γ]< wl >)
+    (VF : [ Γ ||-v< one > F | VΓ ]< wl >)
+    (VU : [ Γ ,, F ||-v< one > U | validSnoc' VΓ VF ]< wl >)
+    (VFU : [ Γ ||-v< one > F : U | VΓ | UValid VΓ ]< wl >)
+    (VGU : [ Γ ,, F ||-v< one > G : U | validSnoc' VΓ VF | VU ]< wl >) .
     (* (VF := univValid (l':=zero) _ _ vFU)
     (VG := univValid (l':=zero) _ _ vGU). *)
 
-  Lemma prodTyEqU {Δ σ σ'} (tΔ : [ |-[ ta ] Δ])
-    (Vσ : [VΓ | Δ ||-v σ : _ | tΔ])
-    (Vσ' : [VΓ | Δ ||-v σ' : _ | tΔ])
-    (Vσσ' : [VΓ | Δ ||-v σ ≅ σ' : _ | tΔ | Vσ ])
-    : [Δ |-[ ta ] tProd F[σ] G[up_term_term σ] ≅ tProd F[σ'] G[up_term_term σ'] : U].
+  Lemma prodTyEqU {Δ σ σ' wl' f} (tΔ : [ |-[ ta ] Δ]< wl' >)
+    (Vσ : [VΓ | Δ ||-v σ : _ | tΔ | f]< wl >)
+    (Vσ' : [VΓ | Δ ||-v σ' : _ | tΔ | f]< wl >)
+    (Vσσ' : [VΓ | Δ ||-v σ ≅ σ' : _ | tΔ | Vσ | f ]< wl >)
+    : [Δ |-[ ta ] tProd F[σ] G[up_term_term σ] ≅ tProd F[σ'] G[up_term_term σ'] : U]< wl' >.
   Proof.
     pose proof (Vuσ := liftSubstS' VF Vσ).
     pose proof (Vureaσ' := liftSubstSrealign' VF Vσσ' Vσ').
     pose proof (Vuσσ' := liftSubstSEq' VF Vσσ').
-    instAllValid Vσ Vσ' Vσσ'; instAllValid Vuσ Vureaσ' Vuσσ'; escape.
+    instAllValid Vσ Vσ' Vσσ'; instAllValid Vuσ Vureaσ' Vuσσ' ; Wescape.
     eapply convtm_prod; tea.
   Qed.
 
-  Lemma PiRedU {Δ σ} (tΔ : [ |-[ ta ] Δ]) (Vσ : [VΓ | Δ ||-v σ : _ | tΔ])
-    : [ Δ ||-< one > (tProd F G)[σ] : U | validTy (UValid VΓ) tΔ Vσ ].
+  Lemma PiRedU {Δ σ wl' f} (tΔ : [ |-[ ta ] Δ]< wl' >) (Vσ : [VΓ | Δ ||-v σ : _ | tΔ | f]< wl >)
+    : W[ Δ ||-< one > (tProd F G)[σ] : U | validTy (UValid VΓ) f tΔ Vσ ]< wl' >.
   Proof.
-    pose proof (Vσσ := reflSubst _ _ Vσ).
+    pose proof (Vσσ := reflSubst _ _ _ Vσ).
     pose proof (Vuσ := liftSubstS' VF Vσ).
     pose proof (Vuσσ := liftSubstSEq' VF Vσσ).
-    instAllValid Vσ Vσ Vσσ; instAllValid Vuσ Vuσ Vuσσ; escape.
+    instAllValid Vσ Vσ Vσσ; instAllValid Vuσ Vuσ Vuσσ; Wescape.
+    econstructor ; intros wl'' Hover Hover'.
     econstructor; cbn.
-    - apply redtmwf_refl; cbn in *; now eapply ty_prod.
+    - apply redtmwf_refl; cbn in *. eapply ty_Ltrans ; [now eapply over_tree_le | ].
+      now eapply ty_prod.
     - constructor.
-    - now eapply convtm_prod.
-    - cbn. unshelve refine (LRCumulative (PiRed _ _ _ tΔ Vσ));
-      unshelve eapply univValid; tea; try irrValid.
+    - eapply convtm_Ltrans ; [now eapply over_tree_le | ].
+      now eapply convtm_prod.
+    - cbn. unshelve refine (WRed _ (WLRCumulative (PiRed _ _ _ _ tΔ Vσ)) _ _). 
+      1: unshelve eapply univValid; tea; try irrValid.
+      1: unshelve eapply univValid; tea; try irrValid.
+      exact Hover'.
   Defined.
 
-  Lemma PiValidU : [ Γ ||-v< one > tProd F G : U | VΓ | UValid VΓ ].
+  Lemma PiValidU : [ Γ ||-v< one > tProd F G : U | VΓ | UValid VΓ ]< wl >.
   Proof.
     econstructor.
-    - intros Δ σ tΔ Vσ.
+    - intros Δ wl' σ f tΔ Vσ.
       exact (PiRedU tΔ Vσ).
-    - intros Δ σ σ' tΔ Vσ Vσ' Vσσ'.
+    - intros Δ wl' σ σ' f tΔ Vσ Vσ' Vσσ'.
       pose proof (univValid (l' := zero) _ _ VFU) as VF0.
-      pose proof (irrelevanceTy (validSnoc VΓ VF)
-                    (validSnoc (l := zero) VΓ VF0)
+      pose proof (irrelevanceTy (validSnoc' VΓ VF)
+                    (validSnoc' (l := zero) VΓ VF0)
                     (univValid (l' := zero) _ _ VGU)) as VG0.
+      pose proof (Help := PiEqRed1 VΓ VF0 VG0 tΔ Vσ Vσ' Vσσ').
+      econstructor ; intros.
       unshelve econstructor ; cbn.
-      + exact (PiRedU tΔ Vσ).
-      + exact (PiRedU tΔ Vσ').
-      + exact (LRCumulative (PiRed VΓ VF0 VG0 tΔ Vσ)).
-      + exact (prodTyEqU tΔ Vσ Vσ' Vσσ').
-      + exact (LRCumulative (PiRed VΓ VF0 VG0 tΔ Vσ')).
-      + pose proof (PiEqRed1 VΓ VF0 VG0 tΔ Vσ Vσ' Vσσ').
-        irrelevanceCum.
+      + eapply (PiRedU tΔ Vσ), over_tree_fusion_l, over_tree_fusion_l ; exact Hover'.
+      + eapply (PiRedU tΔ Vσ'), over_tree_fusion_r, over_tree_fusion_l ; exact Hover'.
+      + unshelve eapply PiRedU ; cycle 1 ; try eassumption.
+        do 2 (eapply over_tree_fusion_l) ; exact Hover'.
+      + cbn ; eapply convtm_Ltrans; [ now eapply over_tree_le | ]. 
+        exact (prodTyEqU tΔ Vσ Vσ' Vσσ').
+      + unshelve eapply PiRedU ; cycle 1 ; try eassumption.
+        eapply over_tree_fusion_r, over_tree_fusion_l ; exact Hover'.
+      + cbn ; unshelve eapply LRTyEqIrrelevantCum'. 
+        4: reflexivity.
+        3: eapply Help. 
+        eapply over_tree_fusion_l, over_tree_fusion_r ; exact Hover'.
+        Unshelve.
+        now do 2 (eapply over_tree_fusion_r) ; exact Hover'.
   Qed.
 
 End PiTmValidity.
@@ -299,47 +381,60 @@ End PiTmValidity.
 Section PiTmCongruence.
 
   Context `{GenericTypingProperties}.
-  Context {Γ F G F' G'}
-    (vΓ : [||-v Γ])
-    (vF : [ Γ ||-v< one > F | vΓ ])
-    (vU : [ Γ ,, F ||-v< one > U | validSnoc vΓ vF ])
-    (vFU : [ Γ ||-v< one > F : U | vΓ | UValid vΓ ])
-    (vGU : [ Γ ,, F ||-v< one > G : U | validSnoc vΓ vF | vU ])
-    (vF' : [ Γ ||-v< one > F' | vΓ ])
-    (vU' : [ Γ ,, F' ||-v< one > U | validSnoc vΓ vF' ])
-    (vF'U : [ Γ ||-v< one > F' : U | vΓ | UValid vΓ ])
-    (vG'U : [ Γ ,, F' ||-v< one > G' : U | validSnoc vΓ vF' | vU' ])
-    (vFF' : [ Γ ||-v< one > F ≅ F' : U | vΓ | UValid vΓ ])
-    (vGG' : [ Γ ,, F ||-v< one > G ≅ G' : U | validSnoc vΓ vF | vU ]).
+  Context {wl Γ F G F' G'}
+    (vΓ : [||-v Γ]< wl >)
+    (vF : [ Γ ||-v< one > F | vΓ ]< wl >)
+    (vU : [ Γ ,, F ||-v< one > U | validSnoc' vΓ vF ]< wl >)
+    (vFU : [ Γ ||-v< one > F : U | vΓ | UValid vΓ ]< wl >)
+    (vGU : [ Γ ,, F ||-v< one > G : U | validSnoc' vΓ vF | vU ]< wl >)
+    (vF' : [ Γ ||-v< one > F' | vΓ ]< wl >)
+    (vU' : [ Γ ,, F' ||-v< one > U | validSnoc' vΓ vF' ]< wl >)
+    (vF'U : [ Γ ||-v< one > F' : U | vΓ | UValid vΓ ]< wl >)
+    (vG'U : [ Γ ,, F' ||-v< one > G' : U | validSnoc' vΓ vF' | vU' ]< wl >)
+    (vFF' : [ Γ ||-v< one > F ≅ F' : U | vΓ | UValid vΓ ]< wl >)
+    (vGG' : [ Γ ,, F ||-v< one > G ≅ G' : U | validSnoc' vΓ vF | vU ]< wl >).
 
-  Lemma PiCongTm : [ Γ ||-v< one > tProd F G ≅ tProd F' G' : U | vΓ | UValid vΓ ].
+  Lemma PiCongTm : [ Γ ||-v< one > tProd F G ≅ tProd F' G' : U | vΓ | UValid vΓ ]< wl >.
   Proof.
     econstructor.
-    intros Δ σ tΔ Vσ.
+    intros Δ wl' σ f tΔ Vσ.
     pose proof (univValid (l' := zero) _ _ vFU) as vF0.
     pose proof (univValid (l' := zero) _ _ vF'U) as vF'0.
-    pose proof (Vσσ := reflSubst _ _ Vσ).
+    pose proof (Vσσ := reflSubst _ _ _ Vσ).
     pose proof (Vuσ := liftSubstS' vF Vσ).
     pose proof (Vuσσ := liftSubstSEq' vF Vσσ).
-    instAllValid Vσ Vσ Vσσ; instAllValid Vuσ Vuσ Vuσσ; escape.
-    pose proof (irrelevanceTy (validSnoc vΓ vF)
-                  (validSnoc (l := zero) vΓ vF0)
+    instAllValid Vσ Vσ Vσσ; instAllValid Vuσ Vuσ Vuσσ; Wescape.
+    pose proof (irrelevanceTy (validSnoc' vΓ vF)
+                  (validSnoc' (l := zero) vΓ vF0)
                   (univValid (l' := zero) _ _ vGU)) as vG0.
-    pose proof (irrelevanceTy (validSnoc vΓ vF')
-                  (validSnoc (l := zero) vΓ vF'0)
+    pose proof (irrelevanceTy (validSnoc' vΓ vF')
+                  (validSnoc' (l := zero) vΓ vF'0)
                   (univValid (l' := zero) _ _ vG'U)) as vG'0.
+    pose proof (univEqValid (validSnoc' vΓ vF) vU (univValid (l' := zero) _ _ vGU) vGG') as vGG'0.
+    epose (Help:= PiEqRed2 vΓ vF0 vG0 vF'0 vG'0 _ _ tΔ Vσ).
+    econstructor ; intros wl'' Hover.
     unshelve econstructor ; cbn.
-    - exact (PiRedU vΓ vF vU vFU vGU tΔ Vσ).
-    - exact (PiRedU vΓ vF' vU' vF'U vG'U tΔ Vσ).
-    - exact (LRCumulative (PiRed vΓ vF0 vG0 tΔ Vσ)).
-    - now eapply convtm_prod.
-    - exact (LRCumulative (PiRed vΓ vF'0 vG'0 tΔ Vσ)).
-    - enough ([ Δ ||-< zero > (tProd F G)[σ] ≅ (tProd F' G')[σ] | PiRed vΓ vF0 vG0 tΔ Vσ]) by irrelevanceCum.
-      refine (PiEqRed2 vΓ vF0 vG0 vF'0 vG'0 _ _ tΔ Vσ).
+    - eapply (PiRedU vΓ vF vU vFU vGU tΔ Vσ).
+      do 2 (eapply over_tree_fusion_l) ; exact Hover'.
+    - eapply (PiRedU vΓ vF' vU' vF'U vG'U tΔ Vσ).
+      eapply over_tree_fusion_r, over_tree_fusion_l ; exact Hover'.
+    - unshelve eapply PiRedU ; cycle 4 ; try eassumption.
+      eapply over_tree_fusion_l, over_tree_fusion_r, over_tree_fusion_r ; exact Hover'.
+    - cbn.
+      eapply convtm_Ltrans ; [eapply over_tree_le ; exact Hover | ].
+      now eapply convtm_prod.
+    - unshelve eapply PiRedU ; cycle 4 ; try eassumption.
+      eapply over_tree_fusion_r, over_tree_fusion_r, over_tree_fusion_r ; exact Hover'.
+    - cbn.
+      unshelve eapply LRTyEqIrrelevantCum'.
+      4: reflexivity.
+      3: unshelve eapply Help.
+      1: eapply over_tree_fusion_l, over_tree_fusion_l, over_tree_fusion_r ; exact Hover'.
+      1: eapply over_tree_fusion_r, over_tree_fusion_l, over_tree_fusion_r ; exact Hover'.
+      Unshelve.
       + exact (univEqValid vΓ (UValid vΓ) vF0 vFF').
-      + pose proof (univEqValid (validSnoc vΓ vF) vU (univValid (l' := zero) _ _ vGU) vGG') as vGG'0.
-        refine (irrelevanceTyEq _ _ _ _ vGG'0).
-  Qed.
+      + refine (irrelevanceTyEq _ _ _ _ vGG'0).
+Qed.
 
 End PiTmCongruence.
 
