theories/Substitution/Introductions/Lambda.v
@@ -1,8 +1,8 @@
 From LogRel.AutoSubst Require Import core unscoped Ast Extra.
-From LogRel Require Import Utils BasicAst Notations Context NormalForms Weakening
-  GenericTyping LogicalRelation Validity.
-From LogRel.LogicalRelation Require Import Escape Reflexivity Neutral Weakening Irrelevance Application Reduction Transitivity NormalRed.
-From LogRel.Substitution Require Import Irrelevance Properties SingleSubst.
+From LogRel Require Import Utils BasicAst Notations LContexts Context NormalForms Weakening
+  GenericTyping Monad LogicalRelation Validity.
+From LogRel.LogicalRelation Require Import Escape Reflexivity Neutral Weakening Monotonicity Irrelevance Application Reduction Transitivity NormalRed.
+From LogRel.Substitution Require Import Irrelevance Monotonicity Properties SingleSubst.
 From LogRel.Substitution.Introductions Require Import Pi.
 
 Set Universe Polymorphism.
@@ -16,9 +16,9 @@ Context `{GenericTypingProperties}.
 
 
 
-Context {Γ F G l} {VΓ : [||-v Γ]} (VF : [Γ ||-v<l> F | VΓ]) 
-  (VΓF := validSnoc VΓ VF)
-  (VG : [Γ ,, F ||-v<l> G | VΓF])
+Context {Γ wl F G l} {VΓ : [||-v Γ]< wl >} (VF : [Γ ||-v<l> F | VΓ]< wl >) 
+  (VΓF := validSnoc' VΓ VF)
+  (VG : [Γ ,, F ||-v<l> G | VΓF]< wl >)
   (VΠFG := PiValid VΓ VF VG).
 
 
@@ -28,72 +28,74 @@ Proof. bsimpl; cbn; now rewrite rinstInst'_term_pointwise. Qed.
 Lemma consWkEq' {Δ Ξ} σ (ρ : Δ ≤ Ξ) a Z : Z[up_term_term σ][a .: ρ >> tRel] = Z[a .: σ⟨ρ⟩].
 Proof. bsimpl; cbn; now rewrite rinstInst'_term_pointwise. Qed.
 
-Lemma lamBetaRed {t} (Vt : [Γ ,, F ||-v<l> t : G | VΓF | VG]) 
-  {Δ σ} (wfΔ : [ |-[ ta ] Δ]) (Vσ : [VΓ | Δ ||-v σ : Γ | wfΔ]) 
-  {Δ0 a} (ρ : Δ0 ≤ Δ) (wfΔ0 : [|-Δ0])
-  (RFσ : [Δ0 ||-<l> F[σ]⟨ρ⟩]) 
-  (ha : [RFσ | _ ||- a : _])
-  (RGσ : [Δ0 ||-<l> G[up_term_term σ][a .: ρ >> tRel]]) :
-    [_ ||-<l> tApp (tLambda F t)[σ]⟨ρ⟩ a : _ | RGσ] × 
-    [_ ||-<l> tApp (tLambda F t)[σ]⟨ρ⟩ a ≅ t[a .: σ⟨ρ⟩] : _ | RGσ].
+Lemma lamBetaRed {t} (Vt : [Γ ,, F ||-v<l> t : G | VΓF | VG]< wl >) 
+  {Δ σ wl' f} (wfΔ : [ |-[ ta ] Δ]< wl' >) (Vσ : [VΓ | Δ ||-v σ : Γ | wfΔ | f]< wl >) 
+  {Δ0 a} (ρ : Δ0 ≤ Δ) (wfΔ0 : [|-Δ0]< wl' >)
+  (RFσ : [Δ0 ||-<l> F[σ]⟨ρ⟩]< wl' >) 
+  (ha : [RFσ | _ ||- a : _]< wl' >)
+  (RGσ : W[Δ0 ||-<l> G[up_term_term σ][a .: ρ >> tRel]]< wl' >) :
+    W[_ ||-<l> tApp (tLambda F t)[σ]⟨ρ⟩ a : _ | RGσ]< wl' > × 
+    W[_ ||-<l> tApp (tLambda F t)[σ]⟨ρ⟩ a ≅ t[a .: σ⟨ρ⟩] : _ | RGσ]< wl' >.
 Proof.
-  pose proof (Vσa := consWkSubstS VF ρ wfΔ0 Vσ ha); instValid Vσa.
+  pose proof (Vσa := consWkSubstS VF ρ wfΔ0 Vσ (TmLogtoW _ ha)); instValid Vσa.
   pose proof (VσUp :=  liftSubstS' VF Vσ).
-  instValid Vσ. instValid VσUp.  escape.
-  irrelevance0. 1: now rewrite consWkEq'.
-  eapply redwfSubstTerm; tea.
-  constructor; tea.
-  do 2 rewrite <- consWkEq.
-  eapply redtm_beta; tea.
-  fold subst_term; renToWk;  eapply ty_wk; tea.
-  eapply wfc_cons; tea; eapply wft_wk; tea.
+  instValid Vσ ; instValid VσUp ; escape ; Wescape.
+  split.
+  all: Wirrelevance0 ; [ now rewrite consWkEq' | ].
+  all: eapply WredwfSubstTerm; tea.
+  all: constructor; tea.
+  all: do 2 rewrite <- consWkEq.
+  all: eapply redtm_beta; tea.
+  all: fold subst_term; renToWk ; eapply ty_wk; tea.
+  all: eapply wfc_cons; tea; eapply wft_wk; tea.
 Qed.
 
-Lemma betaValid {t a} (Vt : [Γ ,, F ||-v<l> t : G | VΓF | VG]) 
-  (Va : [Γ ||-v<l> a : F | VΓ | VF]) :
-  [Γ ||-v<l> tApp (tLambda F t) a ≅ t[a..] : G[a..] | VΓ | substS VG Va].
+Lemma betaValid {t a} (Vt : [Γ ,, F ||-v<l> t : G | VΓF | VG]< wl >) 
+  (Va : [Γ ||-v<l> a : F | VΓ | VF]< wl >) :
+  [Γ ||-v<l> tApp (tLambda F t) a ≅ t[a..] : G[a..] | VΓ | substS VG Va]< wl >.
 Proof.
   constructor; intros. instValid Vσ.
   pose (Vσa := consSubstS _ _ Vσ _ RVa). instValid Vσa.
   pose proof (VσUp :=  liftSubstS' VF Vσ).
-  instValid Vσ. instValid VσUp.  escape.
+  instValid Vσ. instValid VσUp. escape ; Wescape.
   assert (eq : forall t, t[a..][σ] = t[up_term_term σ][a[σ]..]) by (intros; now bsimpl).
   assert (eq' : forall t, t[a..][σ] = t[a[σ].: σ]) by (intros; now bsimpl).
-  irrelevance0. 1: symmetry; apply eq.
-  rewrite eq;  eapply redwfSubstTerm; tea.
-  1: rewrite <- eq; rewrite eq'; irrelevance.
+  Wirrelevance0. 1: symmetry; apply eq.
+  rewrite eq;  eapply WredwfSubstTerm; tea.
+  1: rewrite <- eq; rewrite eq'; Wirrelevance.
   constructor; tea.
   * do 2 (rewrite <- eq; rewrite eq'); tea.
   * eapply redtm_beta; tea.
     Unshelve. 2:rewrite <- eq; now rewrite eq'.
 Qed.
 
-Lemma lamValid0 {t} (Vt : [Γ ,, F ||-v<l> t : G | VΓF | VG]) 
-  {Δ σ} (wfΔ : [ |-[ ta ] Δ]) (Vσ : [VΓ | Δ ||-v σ : Γ | wfΔ]) :
-  [validTy VΠFG wfΔ Vσ | Δ ||- (tLambda F t)[σ] : (tProd F G)[σ]].
+Lemma lamValid0 {t} (Vt : [Γ ,, F ||-v<l> t : G | VΓF | VG]< wl >) 
+  {Δ σ wl' f} (wfΔ : [ |-[ ta ] Δ]< wl' >) (Vσ : [VΓ | Δ ||-v σ : Γ | wfΔ | f]< wl >) :
+  W[Δ ||-< l > (tLambda F t)[σ] : (tProd F G)[σ] | validTy VΠFG f wfΔ Vσ]< wl' >.
 Proof.
   pose proof (VσUp :=  liftSubstS' VF Vσ).
-  instValid Vσ. instValid VσUp. escape.
-  pose (RΠ := normRedΠ RVΠFG); refold.
-  enough [RΠ | Δ ||- (tLambda F t)[σ] : (tProd F G)[σ]] by irrelevance.
-  assert [Δ |- (tLambda F t)[σ] : (tProd F G)[σ]] by (escape; cbn; gen_typing).
-  exists (tLambda F t)[σ]; intros; cbn in *.
-  + now eapply redtmwf_refl.
-  + constructor; cbn; intros.
-    - apply reflLRTyEq.
-    - rewrite Poly.eq_subst_2.
-      irrelevance0; [symmetry; apply Poly.eq_subst_2|].
-      unshelve apply Vt; tea.
-      eapply consSubstS.
-      irrelevance0; [|tea].
-      now bsimpl.
-      Unshelve.
-      now unshelve eapply wkSubstS.
-  + eapply convtm_eta; tea.
-    1,2: constructor; tea; eapply escapeEq, reflLRTyEq.
+  instValid Vσ. instValid VσUp. Wescape ; escape.
+  pose (RΠ := WnormRedΠ RVΠFG); refold.
+  enough W[Δ ||-< l > (tLambda F t)[σ] : (tProd F G)[σ] | RΠ]< wl' > by Wirrelevance.
+  assert [Δ |- (tLambda F t)[σ] : (tProd F G)[σ]]< wl' > by (Wescape; cbn; gen_typing).
+  unshelve econstructor.
+  1: now constructor.
+  intros wl'' Hover Hover' ; cbn.
+  pose proof (f' := over_tree_le Hover).
+  unshelve eexists (tLambda F t)[σ] _ _ ; intros; cbn in *.
+  1: shelve.
+  - do 2 eapply DTree_fusion ; [ .. | eapply DTree_fusion | eapply DTree_fusion].
+    all: shelve.
+  - now eapply redtmwf_refl, ty_Ltrans.
+  - eapply convtm_eta; tea.
+    1,2: now eapply wft_Ltrans.
+    1,3: now eapply ty_Ltrans.
+    1,2: constructor; tea; try now eapply wft_Ltrans.
+    1,4: now eapply convty_Ltrans ; [ eassumption | eapply WescapeEq, WreflLRTyEq].
+    1-4: now eapply ty_Ltrans.
     assert (eqσ : forall Z, Z[up_term_term σ] = Z[up_term_term σ]⟨upRen_term_term S⟩[(tRel 0) ..])
     by (intro; bsimpl; cbn; now rewrite rinstInst'_term_pointwise).
-    assert [Δ,, F[σ] |-[ ta ] tApp (tLambda F[σ] t[up_term_term σ])⟨S⟩ (tRel 0) ⤳*  t[up_term_term σ]⟨upRen_term_term S⟩[(tRel 0)..] : G[up_term_term σ]].
+    assert [Δ,, F[σ] |-[ ta ] tApp (tLambda F[σ] t[up_term_term σ])⟨S⟩ (tRel 0) ⤳*  t[up_term_term σ]⟨upRen_term_term S⟩[(tRel 0)..] : G[up_term_term σ]]< wl' >.
     {
       rewrite (eqσ G). eapply redtm_beta.
       * renToWk; eapply wft_wk; tea; gen_typing.
@@ -101,36 +103,87 @@ Proof.
         eapply wfc_cons; [gen_typing | eapply wft_wk; gen_typing].
       * fold ren_term; refine (ty_var _ (in_here _ _)); gen_typing.
     }
+    eapply convtm_Ltrans ; [eassumption |].
     eapply convtm_exp; tea.
-    - rewrite <- eqσ; tea.
-    - rewrite <- eqσ; tea.
-    - unshelve eapply escapeEq, reflLRTyEq; [|tea].
-    - rewrite <- (eqσ t); eapply escapeEqTerm; now eapply reflLRTmEq.
-  + eapply lamBetaRed; tea. 
-  + pose proof (Vσa := consWkSubstS VF ρ h Vσ ha).
-    pose proof (Vσb := consWkSubstS VF ρ h Vσ hb).
-    assert (Vσab : [_ ||-v _ ≅ (b .: σ⟨ρ⟩) : _ | _ | _ | Vσa]).
-    1:{
-      unshelve eapply consSubstSEq'.
-      2: irrelevance.
-      eapply irrelevanceSubstEq.
-      eapply wkSubstSEq ; eapply reflSubst.
-      Unshelve. all: tea.
-    }
-    eapply LREqTermHelper.
-    1,2: eapply lamBetaRed; tea.
-    - irrelevance0; rewrite consWkEq';[reflexivity|].
-      unshelve eapply validTyExt; cycle 3; tea.
-      Unshelve. rewrite consWkEq'; eapply validTy; tea.
-    - epose proof (validTmExt Vt _ _ Vσb Vσab).
-      irrelevance. now rewrite consWkEq'.
+    + rewrite <- eqσ; tea.
+    + rewrite <- eqσ; tea.
+    + unshelve eapply WescapeEq, WreflLRTyEq; [|tea].
+    + rewrite <- (eqσ t); eapply WescapeEqTerm; now eapply WreflLRTmEq.
+  - cbn.
+    econstructor 1 ; cbn; intros.
+    + apply reflLRTyEq.
+    + rewrite Poly.eq_subst_2.
+      irrelevance0; [symmetry; apply Poly.eq_subst_2|].
+      unshelve eapply (validTm Vt _ h _) ; tea.
+      1: exact (f0 •ε (f' •ε f)).
+      eapply consSubstS ; Wirrelevance0; [|eapply TmLogtoW ; tea].
+      now bsimpl.
+      * eapply over_tree_fusion_l ; exact Ho'.
+      * eapply over_tree_fusion_r ; exact Ho'.
+        Unshelve.
+        1-7: shelve.
+        2,4: eassumption.
+        change ([VΓ | Δ0 ||-v σ⟨ρ⟩ : Γ | h | (f0 •ε f') •ε f ]< wl >).
+        unshelve eapply wkSubstS ; [ | now eapply subst_Ltrans].
+        now eapply wfc_Ltrans ; [exact (f0 •ε f') | ].
+  - cbn in *.
+    set (Helper := PolyRed.posRed _ _ _ _).
+    irrelevance0 ; [ reflexivity | ].
+    unshelve eapply (WRedTm _ (fst (lamBetaRed Vt _ _ _ _ _ ha _))).
+    1: econstructor ; intros wl''' Ho'' ; eapply Helper ; exact Ho''. 
+    all: unfold Helper ; clear Helper ; cbn.
+    + exact ((f0 •ε f') •ε f).
+    + now eapply wfc_Ltrans ; [exact (f0 •ε f') | ].
+    + now eapply subst_Ltrans.
+    + eassumption.
+    + exact Ho.
+    + exact Ho'.
+  - cbn in *.
+    epose  (Vσa := consWkSubstS VF ρ Hd (subst_Ltrans (f0 •ε f') _ Vσ) (TmLogtoW _ ha)).
+    epose  (Vσb := consWkSubstS VF ρ Hd (subst_Ltrans (f0 •ε f') _ Vσ) (TmLogtoW _ hb)).
+    unshelve refine (let Vσab : [_ ||-v _ ≅ (b .: σ⟨ρ⟩) : _ | _ | _ | Vσa | _]< wl > := _ in _).
+    1:{ unshelve eapply consSubstSEq'.
+        1,3: enough (equal : F[σ⟨ρ⟩] = F[σ]⟨ρ⟩) ; [ | now bsimpl].
+        1,2 : Wirrelevance0 ; [rewrite equal ; reflexivity | ].
+        1: eapply TmLogtoW ; exact ha.
+        1: eapply TmEqLogtoW ; exact eq.
+        unshelve eapply irrelevanceSubstEq ; [eassumption | eassumption | ..].
+        2: eapply wkSubstSEq.
+        unshelve eapply reflSubst.
+        Unshelve. 1-6: shelve.
+        4: now eapply subst_Ltrans.
+        all: now eapply wfc_Ltrans ; [exact (f0 •ε f') | ].
+      }
+      eapply LREqTermHelper ; [ irrelevanceRefl | ..].
+    1,2: eapply (WRedTmEq _ (snd (lamBetaRed Vt _ _ _ _ _ _ _))).
+    1: eapply over_tree_fusion_l, over_tree_fusion_l ; exact Hoeq.
+    1: eapply over_tree_fusion_r, over_tree_fusion_l ; exact Hoeq.
+    + irrelevance0; rewrite consWkEq';[reflexivity|].
+      unshelve eapply validTyExt ; cycle 6; tea.
+      1: eapply over_tree_fusion_l, over_tree_fusion_l, over_tree_fusion_r ; exact Hoeq.
+      1: eapply over_tree_fusion_r, over_tree_fusion_l, over_tree_fusion_r ; exact Hoeq.
+      Unshelve.
+      1,2: shelve.
+      1: eapply over_tree_fusion_l, over_tree_fusion_r, over_tree_fusion_r ; exact Hoeq.
+      1: eapply over_tree_fusion_l ; do 3 (eapply over_tree_fusion_r) ; exact Hoeq.
+      1,8: rewrite consWkEq'; eapply validTy; tea.
+      all: try eassumption.
+      2,5: now eapply wfc_Ltrans ; [exact (f0 •ε f') | ].
+      1,3: exact ((f0 •ε f') •ε f).
+      1,2: now eapply subst_Ltrans.
+    + epose (X := validTmExt Vt _ _ _ Vσb Vσab).
+      irrelevance0 ; [ | eapply (WRedTmEq _ X)].
+      1: now rewrite consWkEq'.      
+      1: eapply over_tree_fusion_r ; do 3 (eapply over_tree_fusion_r) ; exact Hoeq.
+      Unshelve.
+      1: eapply over_tree_fusion_l, over_tree_fusion_l, over_tree_fusion_r ; exact Hoeq.
 Qed.
 
-Lemma lamValid {t} (Vt : [Γ ,, F ||-v<l> t : G | VΓF | VG])
+Lemma lamValid {t} (Vt : [Γ ,, F ||-v<l> t : G | VΓF | VG]< wl >)
    :
-    [Γ ||-v<l> tLambda F t : tProd F G | VΓ | VΠFG ].
+    [Γ ||-v<l> tLambda F t : tProd F G | VΓ | VΠFG ]< wl >.
 Proof.
-  opector. 1: now apply lamValid0.
+  opector. 1: intros ;  now apply lamValid0.
   intros.
   pose (VσUp :=  liftSubstS' VF Vσ).
   pose proof (VσUp' :=  liftSubstS' VF Vσ').
@@ -138,13 +191,13 @@ Proof.
   pose proof (VσσUp := liftSubstSEq' VF Vσσ').
   instAllValid Vσ Vσ' Vσσ';  instValid VσUp'; instAllValid VσUp VσUprea VσσUp.
   pose (RΠ := normRedΠ RVΠFG); refold.
-  enough [RΠ | Δ ||- (tLambda F t)[σ] ≅ (tLambda F t)[σ'] : (tProd F G)[σ]] by irrelevance.
+  enough [RΠ | Δ ||- (tLambda F t)[σ] ≅ (tLambda F t)[σ'] : (tProd F G)[σ]]< wl > by irrelevance.
   unshelve econstructor.
-  - change [RΠ | Δ ||- (tLambda F t)[σ] : (tProd F G)[σ]].
+  - change [RΠ | Δ ||- (tLambda F t)[σ] : (tProd F G)[σ]]< wl >.
     eapply normLambda.
     epose (lamValid0 Vt wfΔ Vσ).
     irrelevance.
-  - change [RΠ | Δ ||- (tLambda F t)[σ'] : (tProd F G)[σ]].
+  - change [RΠ | Δ ||- (tLambda F t)[σ'] : (tProd F G)[σ]]< wl >.
     eapply normLambda.
     eapply LRTmRedConv.
     2: epose (lamValid0 Vt wfΔ Vσ'); irrelevance.
@@ -190,14 +243,14 @@ Proof.
         do 2 rewrite <- eqσ ; eapply escapeEqTerm; now eapply validTmExt.
   - refold; cbn; intros.
     pose proof (Vσa := consWkSubstS VF ρ h Vσ ha).
-    assert (ha' : [ _||-<l> a : _| wk ρ h RVF0]).
+    assert (ha' : [ _||-<l> a : _| wk ρ h RVF0]< wl >).
     1: {
       eapply LRTmRedConv; tea.
       irrelevance0; [reflexivity|].
       eapply wkEq; eapply (validTyExt VF); tea.
     }
     pose proof (Vσa' := consWkSubstS VF ρ h Vσ' ha').
-    assert (Vσσa : [_ ||-v _ ≅ (a .: σ'⟨ρ⟩) : _ | _ | _ | Vσa]).
+    assert (Vσσa : [_ ||-v _ ≅ (a .: σ'⟨ρ⟩) : _ | _ | _ | Vσa]< wl >).
     {
       unshelve eapply consSubstSEq'.
       2: eapply reflLRTmEq; irrelevance0; [|exact ha]; now bsimpl.
@@ -216,16 +269,16 @@ Qed.
 
 
 Lemma ηeqEqTermConvNf {σ Δ f} (ρ := @wk1 Γ F)
-  (wfΔ : [|- Δ]) (Vσ : [Δ ||-v σ : Γ | VΓ| wfΔ])
+  (wfΔ : [|- Δ]< wl >) (Vσ : [Δ ||-v σ : Γ | VΓ| wfΔ]< wl >)
   (RΠFG := normRedΠ (validTy VΠFG wfΔ Vσ))
-  (Rf : [Δ ||-<l> f[σ] : (tProd F G)[σ] | RΠFG ]) :
-  [Δ ,, F[σ] |- tApp f⟨ρ⟩[up_term_term σ] (tRel 0) ≅ tApp (PiRedTm.nf Rf)⟨↑⟩ (tRel 0) : G[up_term_term σ]].
+  (Rf : [Δ ||-<l> f[σ] : (tProd F G)[σ] | RΠFG ]< wl >) :
+  [Δ ,, F[σ] |- tApp f⟨ρ⟩[up_term_term σ] (tRel 0) ≅ tApp (PiRedTm.nf Rf)⟨↑⟩ (tRel 0) : G[up_term_term σ]]< wl >.
 Proof.
   refold.
   pose (VσUp :=  liftSubstS' VF Vσ).
   instValid Vσ; instValid VσUp; escape.
   destruct (PiRedTm.red Rf); cbn in *.
-  assert (wfΔF : [|- Δ,, F[σ]]) by gen_typing.
+  assert (wfΔF : [|- Δ,, F[σ]]< wl >) by gen_typing.
   unshelve epose proof (r := PiRedTm.app Rf (@wk1 Δ F[σ]) wfΔF (var0 _ _ _)).
   1: now rewrite wk1_ren_on.
   assumption.
@@ -254,8 +307,8 @@ Proof.
   * unshelve eapply escapeEq, reflLRTyEq; [|tea].
 Qed.
 
-Lemma isLRFun_isWfFun : forall {σ Δ f} (wfΔ : [|- Δ]) (vσ : [Δ ||-v σ : Γ | VΓ | wfΔ]) (RΠFG : [Δ ||-< l > (tProd F G)[σ]])
-  (p : [Δ ||-Π f[σ] : tProd F[σ] G[up_term_term σ] | normRedΠ0 (Induction.invLRΠ RΠFG)]),
+Lemma isLRFun_isWfFun : forall {σ Δ f} (wfΔ : [|- Δ]< wl >) (vσ : [Δ ||-v σ : Γ | VΓ | wfΔ]< wl >) (RΠFG : [Δ ||-< l > (tProd F G)[σ]]< wl >)
+  (p : [Δ ||-Π f[σ] : tProd F[σ] G[up_term_term σ] | normRedΠ0 (Induction.invLRΠ RΠFG)]< wl >),
   isWfFun Δ F[σ] G[up_term_term σ] (PiRedTm.nf p).
 Proof.
 intros.
@@ -269,8 +322,8 @@ destruct isfun as [A t vA vt|]; simpl in *; constructor; tea.
   now unshelve eapply escapeEq, vA.
 + assert (Hrw : forall t, t[tRel 0 .: @wk1 Δ A >> tRel] = t).
   { intros; bsimpl; apply idSubst_term; intros []; reflexivity. }
-  assert [Δ |- F[σ]] by now eapply escape.
-  assert (wfΔF : [|- Δ,, F[σ]]) by now apply wfc_cons.
+  assert [Δ |- F[σ]]< wl > by now eapply escape.
+  assert (wfΔF : [|- Δ,, F[σ]]< wl >) by now apply wfc_cons.
   unshelve eassert (vt0 := vt _ (tRel 0) (@wk1 Δ F[σ]) _ _); tea.
   { eapply var0; [now bsimpl|tea]. }
   eapply escapeTerm in vt0.
@@ -280,11 +333,11 @@ destruct isfun as [A t vA vt|]; simpl in *; constructor; tea.
   assert [Δ |- A].
   { rewrite <- (@wk_id_ren_on Δ).
     unshelve eapply escapeConv, vA; tea. }
-  assert (wfΔA : [|- Δ,, A]) by now apply wfc_cons.
-  assert [Δ |-[ ta ] A ≅ F[σ]].
+  assert (wfΔA : [|- Δ,, A]< wl >) by now apply wfc_cons.
+  assert [Δ |-[ ta ] A ≅ F[σ]]< wl >.
   { rewrite <- (wk_id_ren_on Δ F[σ]), <- (wk_id_ren_on Δ A).
     symmetry; now unshelve eapply escapeEq, vA. }
-  assert [Δ,, A ||-< l > G[up_term_term σ]].
+  assert [Δ,, A ||-< l > G[up_term_term σ]]< wl >.
   { eapply validTy with (wfΔ := wfΔA); tea.
     unshelve econstructor; [shelve|]; cbn.
     apply var0conv; [|tea].
@@ -308,18 +361,18 @@ destruct isfun as [A t vA vt|]; simpl in *; constructor; tea.
 Qed.
 
 Lemma ηeqEqTerm {σ Δ f g} (ρ := @wk1 Γ F)
-  (Vfg : [Γ ,, F ||-v<l> tApp f⟨ρ⟩ (tRel 0) ≅ tApp g⟨ρ⟩ (tRel 0) : G | VΓF | VG ])
-  (wfΔ : [|- Δ]) (Vσ : [Δ ||-v σ : Γ | VΓ| wfΔ])
+  (Vfg : [Γ ,, F ||-v<l> tApp f⟨ρ⟩ (tRel 0) ≅ tApp g⟨ρ⟩ (tRel 0) : G | VΓF | VG ]< wl >)
+  (wfΔ : [|- Δ]< wl >) (Vσ : [Δ ||-v σ : Γ | VΓ| wfΔ]< wl >)
   (RΠFG := validTy VΠFG wfΔ Vσ)
-  (Rf : [Δ ||-<l> f[σ] : (tProd F G)[σ] | RΠFG ])
-  (Rg : [Δ ||-<l> g[σ] : (tProd F G)[σ] | RΠFG ]) :
-  [Δ ||-<l> f[σ] ≅ g[σ] : (tProd F G)[σ] | RΠFG ].
+  (Rf : [Δ ||-<l> f[σ] : (tProd F G)[σ] | RΠFG ]< wl >)
+  (Rg : [Δ ||-<l> g[σ] : (tProd F G)[σ] | RΠFG ]< wl >) :
+  [Δ ||-<l> f[σ] ≅ g[σ] : (tProd F G)[σ] | RΠFG ]< wl >.
 Proof.
   set (RΠ := normRedΠ RΠFG); refold.
-  enough [Δ ||-<l> f[σ] ≅ g[σ] : (tProd F G)[σ] | RΠ ] by irrelevance.
+  enough [Δ ||-<l> f[σ] ≅ g[σ] : (tProd F G)[σ] | RΠ ]< wl > by irrelevance.
   opector.
-  - change [Δ ||-<l> f[σ] : (tProd F G)[σ] | RΠ ]; irrelevance.
-  - change [Δ ||-<l> g[σ] : (tProd F G)[σ] | RΠ ]; irrelevance.
+  - change [Δ ||-<l> f[σ] : (tProd F G)[σ] | RΠ ]< wl >; irrelevance.
+  - change [Δ ||-<l> g[σ] : (tProd F G)[σ] | RΠ ]< wl >; irrelevance.
   - cbn; pose (VσUp :=  liftSubstS' VF Vσ).
     instValid Vσ; instValid VσUp; escape.
     eapply convtm_eta; tea.
@@ -328,13 +381,13 @@ Proof.
     + destruct (PiRedTm.red p); cbn in *; tea.
     + now eapply isLRFun_isWfFun.
     + etransitivity ; [symmetry| etransitivity]; tea; eapply ηeqEqTermConvNf.
-  - match goal with H : [_ ||-Π f[σ] : _ | _] |- _ => rename H into Rfσ end.
-    match goal with H : [_ ||-Π g[σ] : _ | _] |- _ => rename H into Rgσ end.
+  - match goal with H : [_ ||-Π f[σ] : _ | _]< wl > |- _ => rename H into Rfσ end.
+    match goal with H : [_ ||-Π g[σ] : _ | _]< wl > |- _ => rename H into Rgσ end.
     cbn; intros ?? ρ' h ha.
     set (ν := (a .: σ⟨ρ'⟩)).
     pose (Vν := consWkSubstS VF ρ' h Vσ ha).
     instValid Vσ; instValid Vν; escape.
-    assert (wfΔF : [|- Δ,, F[σ]]) by gen_typing.
+    assert (wfΔF : [|- Δ,, F[σ]]< wl >) by gen_typing.
     cbn in *.
     assert (eq : forall t, t⟨ρ⟩[a .: σ⟨ρ'⟩] = t[σ]⟨ρ'⟩) by (intros; unfold ρ; now bsimpl).
     do 2 rewrite eq in RVfg.
@@ -353,10 +406,10 @@ Proof.
 Qed.
 
 Lemma etaeqValid {f g} (ρ := @wk1 Γ F)
-  (Vf : [Γ ||-v<l> f : tProd F G | VΓ | VΠFG ])
-  (Vg : [Γ ||-v<l> g : tProd F G | VΓ | VΠFG ]) 
-  (Vfg : [Γ ,, F ||-v<l> tApp f⟨ρ⟩ (tRel 0) ≅ tApp g⟨ρ⟩ (tRel 0) : G | VΓF | VG ]) :
-  [Γ ||-v<l> f ≅ g : tProd F G | VΓ | VΠFG].
+  (Vf : [Γ ||-v<l> f : tProd F G | VΓ | VΠFG ]< wl >)
+  (Vg : [Γ ||-v<l> g : tProd F G | VΓ | VΠFG ]< wl >) 
+  (Vfg : [Γ ,, F ||-v<l> tApp f⟨ρ⟩ (tRel 0) ≅ tApp g⟨ρ⟩ (tRel 0) : G | VΓF | VG ]< wl >) :
+  [Γ ||-v<l> f ≅ g : tProd F G | VΓ | VΠFG]< wl >.
 Proof.
   constructor; intros ??? Vσ; instValid Vσ; now eapply ηeqEqTerm.
 Qed.
